src/AbstractInterpretationWf.v
@@ -171,23 +171,23 @@ Module Compilers.
                          | eapply UnderLets.wf_Proper_list; [ | | solve [ eauto ] ] ].
         Qed.
 
-        Fixpoint wf_reify (is_let_bound : bool) G {t}
+        Fixpoint wf_reify (annotate_with_state : bool) (is_let_bound : bool) G {t}
           : forall v1 v2 (Hv : @wf_value G t v1 v2)
               s1 s2 (Hs : type.and_for_each_lhs_of_arrow (@abstract_domain_R) s1 s2),
-            UnderLets.wf (fun G' => expr.wf G') G (@reify1 is_let_bound t v1 s1) (@reify2 is_let_bound t v2 s2)
-        with wf_reflect G {t}
+            UnderLets.wf (fun G' => expr.wf G') G (@reify1 annotate_with_state is_let_bound t v1 s1) (@reify2 annotate_with_state is_let_bound t v2 s2)
+        with wf_reflect (annotate_with_state : bool) G {t}
              : forall e1 e2 (He : expr.wf G e1 e2)
                  s1 s2 (Hs : abstract_domain_R s1 s2),
-            @wf_value G t (@reflect1 t e1 s1) (@reflect2 t e2 s2).
+            @wf_value G t (@reflect1 annotate_with_state t e1 s1) (@reflect2 annotate_with_state t e2 s2).
         Proof using annotate_Proper bottom'_Proper.
           all: clear -wf_reflect wf_reify annotate_Proper type_base bottom'_Proper.
           all: pose proof (@bottom_for_each_lhs_of_arrow_Proper); cbv [Proper abstract_domain_R] in *.
           all: destruct t as [t|s d];
             [ clear wf_reify wf_reflect
-            | pose proof (fun G => wf_reflect G s) as wf_reflect_s;
-              pose proof (fun G => wf_reflect G d) as wf_reflect_d;
-              pose proof (fun G => wf_reify false G s) as wf_reify_s;
-              pose proof (fun G => wf_reify false G d) as wf_reify_d;
+            | pose proof (fun G => wf_reflect annotate_with_state G s) as wf_reflect_s;
+              pose proof (fun G => wf_reflect annotate_with_state G d) as wf_reflect_d;
+              pose proof (fun G => wf_reify annotate_with_state false G s) as wf_reify_s;
+              pose proof (fun G => wf_reify annotate_with_state false G d) as wf_reify_d;
               pose proof (@bottom_Proper s);
               clear wf_reify wf_reflect ].
           all: cbn [reify reflect] in *.
@@ -208,9 +208,9 @@ Module Compilers.
                               | [ |- expr.wf _ _ _ ] => constructor
                               | [ He : forall seg G' sv1 sv2, G' = (seg ++ ?G)%list -> _ |- UnderLets.wf _ (?v :: ?G) (UnderLets.splice _ _) (UnderLets.splice _ _) ]
                                 => eapply UnderLets.wf_splice; [ apply (He (cons v nil)) | ]
-                              | [ |- UnderLets.wf _ _ (UnderLets.splice (reify1 _ _ _) _) (UnderLets.splice (reify2 _ _ _) _) ]
+                              | [ |- UnderLets.wf _ _ (UnderLets.splice (reify1 _ _ _ _) _) (UnderLets.splice (reify2 _ _ _ _) _) ]
                                 => eapply UnderLets.wf_splice; [ apply wf_reify_s || apply wf_reify_d | ]
-                              | [ |- wf_value _ (reflect1 _ _) (reflect2 _ _) ] => apply wf_reflect_s || apply wf_reflect_d
+                              | [ |- wf_value _ (reflect1 _ _ _) (reflect2 _ _ _) ] => apply wf_reflect_s || apply wf_reflect_d
                               | [ H : wf_value _ ?x ?y |- wf_value _ ?x ?y ]
                                 => eapply wf_value_Proper_list; [ | eassumption ]
                               | [ H : forall x y, ?R x y -> ?R' (?f x) (?g y) |- ?R' (?f _) (?g _) ]
@@ -259,10 +259,10 @@ Module Compilers.
                          end
                        | break_innermost_match_step ].
 
-        Lemma wf_interp G G' {t} (e1 : @expr (@value_with_lets1) t) (e2 : @expr (@value_with_lets2) t)
+        Lemma wf_interp (annotate_with_state : bool) G G' {t} (e1 : @expr (@value_with_lets1) t) (e2 : @expr (@value_with_lets2) t)
               (Hwf : expr.wf G e1 e2)
               (HGG' : forall t v1 v2, List.In (existT _ t (v1, v2)) G -> wf_value_with_lets G' v1 v2)
-          : wf_value_with_lets G' (interp1 e1) (interp2 e2).
+          : wf_value_with_lets G' (interp1 annotate_with_state e1) (interp2 annotate_with_state e2).
         Proof using annotate_Proper bottom'_Proper interp_ident_Proper.
           revert dependent G'; induction Hwf; intros; cbn [interp];
             try solve [ apply interp_ident_Proper; auto
@@ -270,9 +270,9 @@ Module Compilers.
             wf_interp_t.
         Qed.
 
-        Lemma wf_eval_with_bound' G G' {t} e1 e2 (He : expr.wf G e1 e2) st1 st2 (Hst : type.and_for_each_lhs_of_arrow (@abstract_domain_R) st1 st2)
+        Lemma wf_eval_with_bound' (annotate_with_state : bool) G G' {t} e1 e2 (He : expr.wf G e1 e2) st1 st2 (Hst : type.and_for_each_lhs_of_arrow (@abstract_domain_R) st1 st2)
               (HGG' : forall t v1 v2, List.In (existT _ t (v1, v2)) G -> wf_value_with_lets G' v1 v2)
-          : expr.wf G' (@eval_with_bound'1 t e1 st1) (@eval_with_bound'2 t e2 st2).
+          : expr.wf G' (@eval_with_bound'1 annotate_with_state t e1 st1) (@eval_with_bound'2 annotate_with_state t e2 st2).
         Proof using annotate_Proper bottom'_Proper interp_ident_Proper.
           eapply UnderLets.wf_to_expr, UnderLets.wf_splice.
           { eapply wf_interp; solve [ eauto ]. }
@@ -303,7 +303,6 @@ Module Compilers.
         Context (annotate_ident : forall t, abstract_domain' t -> option (ident (t -> t)))
                 (bottom' : forall A, abstract_domain' A)
                 (abstract_interp_ident : forall t, ident t -> type.interp abstract_domain' t)
-                (update_literal_with_state : forall A : base.type.base, abstract_domain' A -> base.interp A -> base.interp A)
                 (extract_list_state : forall A, abstract_domain' (base.type.list A) -> option (list (abstract_domain' A)))
                 (is_annotated_for : forall t t', ident t -> abstract_domain' t' -> bool).
         Context (abstract_domain'_R : forall t, abstract_domain' t -> abstract_domain' t -> Prop).
@@ -311,7 +310,6 @@ Module Compilers.
         Context {annotate_ident_Proper : forall t, Proper (abstract_domain'_R t ==> eq) (annotate_ident t)}
                 {abstract_interp_ident_Proper : forall t, Proper (eq ==> @abstract_domain_R t) (abstract_interp_ident t)}
                 {bottom'_Proper : forall t, Proper (abstract_domain'_R t) (bottom' t)}
-                {update_literal_with_state_Proper : forall t, Proper (abstract_domain'_R (base.type.type_base t) ==> eq ==> eq) (update_literal_with_state t)}
                 {is_annotated_for_Proper : forall t t', Proper (eq ==> abstract_domain'_R _ ==> eq) (@is_annotated_for t t')}
                 (extract_list_state_length : forall t v1 v2, abstract_domain'_R _ v1 v2 -> option_map (@length _) (extract_list_state t v1) = option_map (@length _) (extract_list_state t v2))
                 (extract_list_state_rel : forall t v1 v2, abstract_domain'_R _ v1 v2 -> forall l1 l2, extract_list_state t v1 = Some l1 -> extract_list_state t v2 = Some l2 -> forall vv1 vv2, List.In (vv1, vv2) (List.combine l1 l2) -> @abstract_domain'_R t vv1 vv2).
@@ -325,14 +323,14 @@ Module Compilers.
 
           Local Notation update_annotation1 := (@ident.update_annotation var1 abstract_domain' annotate_ident is_annotated_for).
           Local Notation update_annotation2 := (@ident.update_annotation var2 abstract_domain' annotate_ident is_annotated_for).
-          Local Notation annotate1 := (@ident.annotate var1 abstract_domain' annotate_ident abstract_interp_ident update_literal_with_state extract_list_state is_annotated_for).
-          Local Notation annotate2 := (@ident.annotate var2 abstract_domain' annotate_ident abstract_interp_ident update_literal_with_state extract_list_state is_annotated_for).
-          Local Notation annotate_base1 := (@ident.annotate_base var1 abstract_domain' annotate_ident update_literal_with_state is_annotated_for).
-          Local Notation annotate_base2 := (@ident.annotate_base var2 abstract_domain' annotate_ident update_literal_with_state is_annotated_for).
+          Local Notation annotate1 := (@ident.annotate var1 abstract_domain' annotate_ident abstract_interp_ident extract_list_state is_annotated_for).
+          Local Notation annotate2 := (@ident.annotate var2 abstract_domain' annotate_ident abstract_interp_ident extract_list_state is_annotated_for).
+          Local Notation annotate_base1 := (@ident.annotate_base var1 abstract_domain' annotate_ident is_annotated_for).
+          Local Notation annotate_base2 := (@ident.annotate_base var2 abstract_domain' annotate_ident is_annotated_for).
           Local Notation annotate_with_ident1 := (@ident.annotate_with_ident var1 abstract_domain' annotate_ident is_annotated_for).
           Local Notation annotate_with_ident2 := (@ident.annotate_with_ident var2 abstract_domain' annotate_ident is_annotated_for).
-          Local Notation interp_ident1 := (@ident.interp_ident var1 abstract_domain' annotate_ident bottom' abstract_interp_ident update_literal_with_state extract_list_state is_annotated_for).
-          Local Notation interp_ident2 := (@ident.interp_ident var2 abstract_domain' annotate_ident bottom' abstract_interp_ident update_literal_with_state extract_list_state is_annotated_for).
+          Local Notation interp_ident1 := (@ident.interp_ident var1 abstract_domain' annotate_ident bottom' abstract_interp_ident extract_list_state is_annotated_for).
+          Local Notation interp_ident2 := (@ident.interp_ident var2 abstract_domain' annotate_ident bottom' abstract_interp_ident extract_list_state is_annotated_for).
           Local Notation reflect1 := (@reflect base.type ident var1 abstract_domain' annotate1 bottom').
           Local Notation reflect2 := (@reflect base.type ident var2 abstract_domain' annotate2 bottom').
 
@@ -382,7 +380,7 @@ Module Compilers.
                 v1 v2 (Hv : abstract_domain'_R t v1 v2)
                 e1 e2 (He : expr.wf G e1 e2)
             : UnderLets.wf (fun G' => expr.wf G') G (@annotate_base1 is_let_bound t v1 e1) (@annotate_base2 is_let_bound t v2 e2).
-          Proof using abstract_interp_ident_Proper annotate_ident_Proper update_literal_with_state_Proper is_annotated_for_Proper.
+          Proof using abstract_interp_ident_Proper annotate_ident_Proper is_annotated_for_Proper.
             cbv [ident.annotate_base];
               repeat first [ apply wf_annotate_with_ident
                            | break_innermost_match_step
@@ -409,7 +407,7 @@ Module Compilers.
                 v1 v2 (Hv : abstract_domain'_R t v1 v2)
                 e1 e2 (He : expr.wf G e1 e2)
             : UnderLets.wf (fun G' => expr.wf G') G (@annotate1 is_let_bound t v1 e1) (@annotate2 is_let_bound t v2 e2).
-          Proof using abstract_interp_ident_Proper annotate_ident_Proper extract_list_state_length extract_list_state_rel update_literal_with_state_Proper is_annotated_for_Proper.
+          Proof using abstract_interp_ident_Proper annotate_ident_Proper extract_list_state_length extract_list_state_rel is_annotated_for_Proper.
             revert dependent G; induction t; intros;
               cbn [ident.annotate]; try apply wf_annotate_base; trivial.
             all: repeat first [ lazymatch goal with
@@ -491,9 +489,9 @@ Module Compilers.
                 let b' := type_of_value b in
                 constr:(type.arrow a' b')
             end.
-          Lemma wf_interp_ident_nth_default G T
-            : wf_value_with_lets G (@interp_ident1 _ (@ident.List_nth_default T)) (@interp_ident2 _ (@ident.List_nth_default T)).
-          Proof using abstract_interp_ident_Proper annotate_ident_Proper extract_list_state_length extract_list_state_rel update_literal_with_state_Proper is_annotated_for_Proper.
+          Lemma wf_interp_ident_nth_default (annotate_with_state : bool) G T
+            : wf_value_with_lets G (@interp_ident1 annotate_with_state _ (@ident.List_nth_default T)) (@interp_ident2 annotate_with_state _ (@ident.List_nth_default T)).
+          Proof using abstract_interp_ident_Proper annotate_ident_Proper extract_list_state_length extract_list_state_rel is_annotated_for_Proper.
             cbv [wf_value_with_lets wf_value ident.interp_ident]; constructor; cbn -[abstract_domain_R abstract_domain].
             { intros; subst.
               destruct_head'_prod; destruct_head'_and; cbn [fst snd] in *.
@@ -599,9 +597,9 @@ Module Compilers.
                              end ]. }
           Qed.
 
-          Lemma wf_interp_ident_not_nth_default G {t} (idc : ident t)
-            : wf_value_with_lets G (Base (reflect1 (###idc)%expr (abstract_interp_ident _ idc))) (Base (reflect2 (###idc)%expr (abstract_interp_ident _ idc))).
-          Proof using abstract_interp_ident_Proper annotate_ident_Proper bottom'_Proper extract_list_state_length extract_list_state_rel update_literal_with_state_Proper is_annotated_for_Proper.
+          Lemma wf_interp_ident_not_nth_default (annotate_with_state : bool) G {t} (idc : ident t)
+            : wf_value_with_lets G (Base (reflect1 annotate_with_state (###idc)%expr (abstract_interp_ident _ idc))) (Base (reflect2 annotate_with_state (###idc)%expr (abstract_interp_ident _ idc))).
+          Proof using abstract_interp_ident_Proper annotate_ident_Proper bottom'_Proper extract_list_state_length extract_list_state_rel is_annotated_for_Proper.
             constructor; eapply wf_reflect;
               solve [ apply bottom'_Proper
                     | apply wf_annotate
@@ -609,43 +607,43 @@ Module Compilers.
                     | apply abstract_interp_ident_Proper; reflexivity ].
           Qed.
 
-          Lemma wf_interp_ident G {t} idc1 idc2 (Hidc : idc1 = idc2)
-            : wf_value_with_lets G (@interp_ident1 t idc1) (@interp_ident2 t idc2).
-          Proof using abstract_interp_ident_Proper annotate_ident_Proper bottom'_Proper extract_list_state_length extract_list_state_rel update_literal_with_state_Proper is_annotated_for_Proper.
+          Lemma wf_interp_ident (annotate_with_state : bool) G {t} idc1 idc2 (Hidc : idc1 = idc2)
+            : wf_value_with_lets G (@interp_ident1 annotate_with_state t idc1) (@interp_ident2 annotate_with_state t idc2).
+          Proof using abstract_interp_ident_Proper annotate_ident_Proper bottom'_Proper extract_list_state_length extract_list_state_rel is_annotated_for_Proper.
             cbv [wf_value_with_lets ident.interp_ident]; subst idc2; destruct idc1;
               first [ apply wf_interp_ident_nth_default
                     | apply wf_interp_ident_not_nth_default ].
           Qed.
 
-          Local Notation eval_with_bound1 := (@partial.ident.eval_with_bound var1 abstract_domain' annotate_ident bottom' abstract_interp_ident update_literal_with_state extract_list_state is_annotated_for).
-          Local Notation eval_with_bound2 := (@partial.ident.eval_with_bound var2 abstract_domain' annotate_ident bottom' abstract_interp_ident update_literal_with_state extract_list_state is_annotated_for).
-          Lemma wf_eval_with_bound {t} G G' e1 e2 (Hwf : expr.wf G e1 e2) st1 st2 (Hst : type.and_for_each_lhs_of_arrow (@abstract_domain_R) st1 st2)
+          Local Notation eval_with_bound1 := (@partial.ident.eval_with_bound var1 abstract_domain' annotate_ident bottom' abstract_interp_ident extract_list_state is_annotated_for).
+          Local Notation eval_with_bound2 := (@partial.ident.eval_with_bound var2 abstract_domain' annotate_ident bottom' abstract_interp_ident extract_list_state is_annotated_for).
+          Lemma wf_eval_with_bound (annotate_with_state : bool) {t} G G' e1 e2 (Hwf : expr.wf G e1 e2) st1 st2 (Hst : type.and_for_each_lhs_of_arrow (@abstract_domain_R) st1 st2)
                 (HGG' : forall t v1 v2, List.In (existT _ t (v1, v2)) G -> wf_value_with_lets G' v1 v2)
-            : expr.wf G' (@eval_with_bound1 t e1 st1) (@eval_with_bound2 t e2 st2).
-          Proof using abstract_interp_ident_Proper annotate_ident_Proper bottom'_Proper extract_list_state_length extract_list_state_rel update_literal_with_state_Proper is_annotated_for_Proper.
+            : expr.wf G' (@eval_with_bound1 annotate_with_state t e1 st1) (@eval_with_bound2 annotate_with_state t e2 st2).
+          Proof using abstract_interp_ident_Proper annotate_ident_Proper bottom'_Proper extract_list_state_length extract_list_state_rel is_annotated_for_Proper.
             eapply wf_eval_with_bound';
               solve [ eassumption
                     | eapply wf_annotate
                     | eapply wf_interp_ident ].
           Qed.
 
-          Local Notation eval1 := (@partial.ident.eval var1 abstract_domain' annotate_ident bottom' abstract_interp_ident update_literal_with_state extract_list_state is_annotated_for).
-          Local Notation eval2 := (@partial.ident.eval var2 abstract_domain' annotate_ident bottom' abstract_interp_ident update_literal_with_state extract_list_state is_annotated_for).
+          Local Notation eval1 := (@partial.ident.eval var1 abstract_domain' annotate_ident bottom' abstract_interp_ident extract_list_state is_annotated_for).
+          Local Notation eval2 := (@partial.ident.eval var2 abstract_domain' annotate_ident bottom' abstract_interp_ident extract_list_state is_annotated_for).
           Lemma wf_eval {t} G G' e1 e2 (Hwf : expr.wf G e1 e2)
                 (HGG' : forall t v1 v2, List.In (existT _ t (v1, v2)) G -> wf_value_with_lets G' v1 v2)
             : expr.wf G' (@eval1 t e1) (@eval2 t e2).
-          Proof using abstract_interp_ident_Proper annotate_ident_Proper bottom'_Proper extract_list_state_length extract_list_state_rel update_literal_with_state_Proper is_annotated_for_Proper.
+          Proof using abstract_interp_ident_Proper annotate_ident_Proper bottom'_Proper extract_list_state_length extract_list_state_rel is_annotated_for_Proper.
             eapply wf_eval';
               solve [ eassumption
                     | eapply wf_annotate
                     | eapply wf_interp_ident ].
           Qed.
 
-          Local Notation eta_expand_with_bound1 := (@partial.ident.eta_expand_with_bound var1 abstract_domain' annotate_ident bottom' abstract_interp_ident update_literal_with_state extract_list_state is_annotated_for).
-          Local Notation eta_expand_with_bound2 := (@partial.ident.eta_expand_with_bound var2 abstract_domain' annotate_ident bottom' abstract_interp_ident update_literal_with_state extract_list_state is_annotated_for).
+          Local Notation eta_expand_with_bound1 := (@partial.ident.eta_expand_with_bound var1 abstract_domain' annotate_ident bottom' abstract_interp_ident extract_list_state is_annotated_for).
+          Local Notation eta_expand_with_bound2 := (@partial.ident.eta_expand_with_bound var2 abstract_domain' annotate_ident bottom' abstract_interp_ident extract_list_state is_annotated_for).
           Lemma wf_eta_expand_with_bound {t} G e1 e2 (Hwf : expr.wf G e1 e2) st1 st2 (Hst : type.and_for_each_lhs_of_arrow (@abstract_domain_R) st1 st2)
             : expr.wf G (@eta_expand_with_bound1 t e1 st1) (@eta_expand_with_bound2 t e2 st2).
-          Proof using abstract_interp_ident_Proper annotate_ident_Proper bottom'_Proper extract_list_state_length extract_list_state_rel update_literal_with_state_Proper is_annotated_for_Proper.
+          Proof using abstract_interp_ident_Proper annotate_ident_Proper bottom'_Proper extract_list_state_length extract_list_state_rel is_annotated_for_Proper.
             eapply wf_eta_expand_with_bound';
               solve [ eassumption
                     | eapply wf_annotate
@@ -696,10 +694,6 @@ Module Compilers.
                          | [ H : _ |- _ ] => erewrite H by (eauto; (eassumption || reflexivity))
                          end ].
       Qed.
-
-      Global Instance update_literal_with_state_Proper {t}
-        : Proper (abstract_domain'_R (base.type.type_base t) ==> eq ==> eq) (update_literal_with_state t).
-      Proof. repeat intro; congruence. Qed.
 
       Global Instance extract_list_state_Proper {t}
         : Proper (abstract_domain'_R _ ==> option_eq (SetoidList.eqlistA (@abstract_domain'_R t)))
